FypSchedulingAlgorithms.lean
@@ -3,5 +3,6 @@ import FypSchedulingAlgorithms.SchedState
 import FypSchedulingAlgorithms.Step
 import FypSchedulingAlgorithms.Test
 import FypSchedulingAlgorithms.AperiodicSchedulers.AperiodicStep
-import FypSchedulingAlgorithms.AperiodicSchedulers.Starvation
+import FypSchedulingAlgorithms.AperiodicSchedulers.FCFSStarvationFree
+-- import FypSchedulingAlgorithms.AperiodicSchedulers.RRStarvationFree
 import FypSchedulingAlgorithms.PeriodicSchedulers.PeriodicStep
